task 3, 4

hw2.thy
@@ -19,24 +19,25 @@ OD
 {y = fact x}"
   apply vcg_simp
   by (auto simp add: fact_reduce)
+ 
 
 (*2*)
 
-function sum :: "nat \<Rightarrow> nat \<Rightarrow> nat"
+function sum :: "nat ⇒ nat ⇒ nat"
   where "sum i N = (if i > N then 0 else i + sum (Suc i) N)"
   by pat_completeness auto
 termination sum
-  apply (relation "measure (\<lambda>(i,N). N + 1 - i)")
+  apply (relation "measure (λ(i,N). N + 1 - i)")
   apply auto
   done
 
 value "sum 1 2"
 
 lemma SumLemma: "VARS (s :: nat) (i :: nat) 
-{b\<ge>0}
+{b≥0}
 s:=0;
 i:=a;
-WHILE i \<le> b
+WHILE i ≤ b
 INV { sum a b = s + sum i b }
 DO
 s := s + i; 
@@ -47,6 +48,38 @@ OD
   done
 
 (*3*)
+
+function perm::"nat list ⇒ nat list ⇒ bool" 
+  where "perm [] [] = True" |
+"perm [] (y#ys) = False" |
+"perm (x#xs) ys = (if length (x#xs) ≠ length ys then False 
+                  else perm (removeAll x xs) (removeAll x ys))"
+  apply (metis list.exhaust subset_eq_mset_impl.cases)
+  apply (auto)
+  done
+
+
+(*4*)
+
+datatype tree0 = Node tree0 tree0 | Nil
+
+fun nodes :: "tree0 ⇒ nat" where
+"nodes Nil = 0" |
+"nodes (Node l r) = Suc(nodes l + nodes r)"
+
+fun explode :: "nat ⇒ tree0 ⇒ tree0" where
+"explode 0 t = t"|
+"explode (Suc n) t = explode n (Node t t)"
+
+value "nodes(explode 12 (Node Nil Nil))"
+value "2^(12)*(Suc(nodes (Node Nil Nil)))-1"
+
+lemma "nodes(explode n t) = 2^(n)*(Suc(nodes t)) - 1 "
+  apply(induction n arbitrary: t)
+  apply (auto)
+  by (smt add.assoc  mult.assoc  mult.commute  mult_2_right)
+
+
 (*5*)
 fun itadd::"nat ⇒ nat ⇒ nat"  where 
  "itadd 0 n = n" |
